language/stackless_bytecode/bytecode_to_boogie/src/bytecode_instrs.bpl
@@ -2,6 +2,7 @@ type TypeName;
 type FieldName;
 type LocalName;
 type Address;
+type ByteArray;
 type String;
 type CreationTime = int;
 
@@ -18,6 +19,8 @@ type {:datatype} Value;
 function {:constructor} Boolean(b: bool): Value;
 function {:constructor} Integer(i: int): Value;
 function {:constructor} Address(a: Address): Value;
+function {:constructor} ByteArray(b: ByteArray): Value;
+function {:constructor} Str(a: String): Value;
 function {:constructor} Map(m: [Edge]Value): Value;
 
 const DefaultMap: [Edge]Value;
@@ -76,6 +79,7 @@ procedure {:inline 1} DeepUpdateGlobal(t: TypeName, src: Reference, dst: Resourc
 
 procedure {:inline 1} Exists(address: Value, rs: ResourceStore) returns (dst: Value)
 {
+    assert is#Address(address);
     dst := Boolean(domain#ResourceStore(rs)[a#Address(address)]);
 }
 
@@ -90,6 +94,7 @@ procedure {:inline 1} MoveToSender(rs: ResourceStore, v: Value) returns (rs': Re
 procedure {:inline 1} MoveFrom(address: Value, rs: ResourceStore) returns (dst: Value, rs': ResourceStore)
 {
     var a: Address;
+    assert is#Address(address);
     a := a#Address(address);
     assert domain#ResourceStore(rs)[a];
     dst := contents#ResourceStore(rs)[a];
@@ -114,8 +119,10 @@ procedure {:inline 1} BorrowLoc(c: CreationTime, l: LocalName, local: Value) ret
 procedure {:inline 1} BorrowField(src: Reference, f: FieldName) returns (dst: Reference)
 {
     if (is#GlobalReference(src)) {
+        assert is#Map(v#GlobalReference(src));
         dst := GlobalReference(a#GlobalReference(src), t#GlobalReference(src), Cons(p#GlobalReference(src), Field(f)), m#Map(v#GlobalReference(src))[Field(f)]);
     } else {
+        assert is#Map(v#LocalReference(src));
         dst := LocalReference(c#LocalReference(src), l#LocalReference(src), Cons(p#LocalReference(src), Field(f)), m#Map(v#LocalReference(src))[Field(f)]);
     }
 }
@@ -157,87 +164,130 @@ procedure {:inline 1} FreezeRef(src: Reference) returns (dest: Reference)
 
 procedure {:inline 1} Add(src1: Value, src2: Value) returns (dst: Value)
 {
+    assert is#Integer(src1) && is#Integer(src2);
     dst := Integer(i#Integer(src1) + i#Integer(src2));
 }
 
 procedure {:inline 1} Sub(src1: Value, src2: Value) returns (dst: Value)
 {
+    assert is#Integer(src1) && is#Integer(src2);
     dst := Integer(i#Integer(src1) - i#Integer(src2));
 }
 
 procedure {:inline 1} Mul(src1: Value, src2: Value) returns (dst: Value)
 {
+    assert is#Integer(src1) && is#Integer(src2);
     dst := Integer(i#Integer(src1) * i#Integer(src2));
 }
 
 procedure {:inline 1} Div(src1: Value, src2: Value) returns (dst: Value)
 {
+    assert is#Integer(src1) && is#Integer(src2);
     dst := Integer(i#Integer(src1) div i#Integer(src2));
 }
 
 procedure {:inline 1} Mod(src1: Value, src2: Value) returns (dst: Value)
 {
+    assert is#Integer(src1) && is#Integer(src2);
     dst := Integer(i#Integer(src1) mod i#Integer(src2));
 }
 
 procedure {:inline 1} Lt(src1: Value, src2: Value) returns (dst: Value)
 {
+    assert is#Integer(src1) && is#Integer(src2);
     dst := Boolean(i#Integer(src1) < i#Integer(src2));
 }
 
 procedure {:inline 1} Gt(src1: Value, src2: Value) returns (dst: Value)
 {
+    assert is#Integer(src1) && is#Integer(src2);
     dst := Boolean(i#Integer(src1) > i#Integer(src2));
 }
 
 procedure {:inline 1} Le(src1: Value, src2: Value) returns (dst: Value)
 {
+    assert is#Integer(src1) && is#Integer(src2);
     dst := Boolean(i#Integer(src1) <= i#Integer(src2));
 }
 
 procedure {:inline 1} Ge(src1: Value, src2: Value) returns (dst: Value)
 {
+    assert is#Integer(src1) && is#Integer(src2);
     dst := Boolean(i#Integer(src1) >= i#Integer(src2));
 }
 
 procedure {:inline 1} And(src1: Value, src2: Value) returns (dst: Value)
 {
+    assert is#Boolean(src1) && is#Boolean(src2);
     dst := Boolean(b#Boolean(src1) && b#Boolean(src2));
 }
 
 procedure {:inline 1} Or(src1: Value, src2: Value) returns (dst: Value)
 {
+    assert is#Boolean(src1) && is#Boolean(src2);
     dst := Boolean(b#Boolean(src1) || b#Boolean(src2));
 }
 
 procedure {:inline 1} Not(src: Value) returns (dst: Value)
 {
+    assert is#Boolean(src);
     dst := Boolean(!b#Boolean(src));
 }
 
 procedure {:inline 1} Eq_int(src1: Value, src2: Value) returns (dst: Value)
 {
+    assert is#Integer(src1) && is#Integer(src2);
     dst := Boolean(i#Integer(src1) == i#Integer(src2));
 }
 
 procedure {:inline 1} Neq_int(src1: Value, src2: Value) returns (dst: Value)
 {
+    assert is#Integer(src1) && is#Integer(src2);
     dst := Boolean(i#Integer(src1) != i#Integer(src2));
 }
 
 procedure {:inline 1} Eq_bool(src1: Value, src2: Value) returns (dst: Value)
 {
+    assert is#Boolean(src1) && is#Boolean(src2);
     dst := Boolean(b#Boolean(src1) == b#Boolean(src2));
 }
 
 procedure {:inline 1} Neq_bool(src1: Value, src2: Value) returns (dst: Value)
 {
+    assert is#Boolean(src1) && is#Boolean(src2);
     dst := Boolean(b#Boolean(src1) != b#Boolean(src2));
+}
+
+procedure {:inline 1} Eq_address(src1: Value, src2: Value) returns (dst: Value)
+{
+    assert is#Address(src1) && is#Address(src2);
+    dst := Boolean(a#Address(src1) == a#Address(src2));
+}
+
+procedure {:inline 1} Neq_address(src1: Value, src2: Value) returns (dst: Value)
+{
+    assert is#Address(src1) && is#Address(src2);
+    dst := Boolean(a#Address(src1) != a#Address(src2));
 }
 
 procedure {:inline 1} LdConst(val: int) returns (ret: Value)
 {
     ret := Integer(val);
+}
+
+procedure {:inline 1} LdAddr(val: Address) returns (ret: Value)
+{
+    ret := Address(val);
+}
+
+procedure {:inline 1} LdByteArray(val: ByteArray) returns (ret: Value)
+{
+    ret := ByteArray(val);
+}
+
+procedure {:inline 1} LdStr(val: String) returns (ret: Value)
+{
+    ret := Str(val);
 }
 
 procedure {:inline 1} LdTrue() returns (ret: Value)
@@ -248,4 +298,52 @@ procedure {:inline 1} LdTrue() returns (ret: Value)
 procedure {:inline 1} LdFalse() returns (ret: Value)
 {
     ret := Boolean(false);
+}
+
+// Transaction builtin instructions
+type {:datatype} Transaction;
+var txn: Transaction;
+function {:constructor} Transaction_cons(
+  gas_unit_price: int, max_gas_units: int, public_key: ByteArray,
+  sender: Address, sequence_number: int, gas_remaining: int) : Transaction;
+
+procedure {:inline 1} GetGasRemaining() returns (ret_gas_remaining: Value)
+{
+  ret_gas_remaining := Integer(gas_remaining#Transaction_cons(txn));
+}
+
+procedure {:inline 1} GetTxnSequenceNumber() returns (ret_sequence_number: Value)
+{
+  ret_sequence_number := Integer(sequence_number#Transaction_cons(txn));
+}
+
+procedure {:inline 1} GetTxnPublicKey() returns (ret_public_key: Value)
+{
+  ret_public_key := ByteArray(public_key#Transaction_cons(txn));
+}
+
+procedure {:inline 1} GetTxnSenderAddress() returns (ret_sender: Value)
+{
+  ret_sender := Address(sender#Transaction_cons(txn));
+}
+
+procedure {:inline 1} GetTxnMaxGasUnits() returns (ret_max_gas_units: Value)
+{
+  ret_max_gas_units := Integer(max_gas_units#Transaction_cons(txn));
+}
+
+procedure {:inline 1} GetTxnGasUnitPrice() returns (ret_gas_unit_price: Value)
+{
+  ret_gas_unit_price := Integer(gas_unit_price#Transaction_cons(txn));
+}
+
+// Special instruction
+var Address_Exists: [Address]bool;
+procedure {:inline 1} CreateAccount(addr_val: Value)
+modifies Address_Exists;
+{
+  var addr: Address;
+  addr := a#Address(addr_val);
+  assert !Address_Exists[addr];
+  Address_Exists[addr] := true;
 }
